src/coq/Handlers/MemoryModel.v
@@ -19,7 +19,8 @@ From Vellvm.Utils Require Import
      PropT
      Util
      NMaps
-     Tactics.
+     Tactics
+     MonadReturnsLaws.
 
 From Vellvm.Numeric Require Import
      Integers.
@@ -67,6 +68,10 @@ Module Type MemoryModelSpecPrimitives (LP : LLVMParams) (MP : MemoryParams LP).
 
   (*** Internal state of memory *)
   Parameter MemState : Type.
+  Parameter memory_stack : Type.
+  Parameter MemState_get_memory : MemState -> memory_stack.
+  Parameter MemState_get_provenance : MemState -> Provenance.
+  Parameter MemState_put_memory : memory_stack -> MemState -> MemState.
 
   (* Type for frames and frame stacks *)
   Parameter Frame : Type.
@@ -86,11 +91,11 @@ Module Type MemoryModelSpecPrimitives (LP : LLVMParams) (MP : MemoryParams LP).
   (*** Primitives on memory *)
 
   (** Reads *)
-  Parameter read_byte_MemPropT : addr -> MemPropT MemState SByte.
+  Parameter read_byte_MemPropT : addr -> MemPropT memory_stack SByte.
 
   (** Allocations *)
   (* Returns true if a byte is allocated with a given AllocationId? *)
-  Parameter addr_allocated_prop : addr -> AllocationId -> MemPropT MemState bool.
+  Parameter addr_allocated_prop : addr -> AllocationId -> MemPropT memory_stack bool.
 
   (** Frame stacks *)
   (* Check if an address is allocated in a frame *)
@@ -100,7 +105,7 @@ Module Type MemoryModelSpecPrimitives (LP : LLVMParams) (MP : MemoryParams LP).
   Parameter peek_frame_stack_prop : FrameStack -> Frame -> Prop.
   Parameter pop_frame_stack_prop : FrameStack -> FrameStack -> Prop.
 
-  Parameter mem_state_frame_stack_prop : MemState -> FrameStack -> Prop.
+  Parameter mem_state_frame_stack_prop : memory_stack -> FrameStack -> Prop.
 
   Definition frame_eqv (f f' : Frame) : Prop :=
     forall ptr, ptr_in_frame_prop f ptr <-> ptr_in_frame_prop f' ptr.
@@ -128,7 +133,14 @@ Module Type MemoryModelSpecPrimitives (LP : LLVMParams) (MP : MemoryParams LP).
   Parameter mem_state_fresh_provenance_fresh :
     forall (ms ms' : MemState) (pr : Provenance),
       mem_state_fresh_provenance ms = (pr, ms') ->
+      MemState_get_memory ms = MemState_get_memory ms' /\
       ~ used_provenance_prop ms pr /\ used_provenance_prop ms' pr.
+
+  (** Lemmas about MemState *)
+  Parameter MemState_get_put_memory :
+    forall ms mem,
+      MemState_get_memory (MemState_put_memory mem ms) = mem.
+
 End MemoryModelSpecPrimitives.
 
 Module MemoryHelpers (LP : LLVMParams) (MP : MemoryParams LP) (Byte : ByteModule LP.ADDR LP.IP LP.SIZEOF LP.Events MP.BYTE_IMPL).
@@ -962,11 +974,16 @@ Module Type MemoryModelSpec (LP : LLVMParams) (MP : MemoryParams LP) (MMSP : Mem
   Import MemHelpers.
 
   Definition read_byte_prop (ms : MemState) (ptr : addr) (byte : SByte) : Prop
-    := read_byte_MemPropT ptr ms (ret (ms, byte)).
+    := read_byte_MemPropT ptr (MemState_get_memory ms) (ret ((MemState_get_memory ms), byte)).
+
+  Definition lift_memory_MemPropT {X} (m : MemPropT memory_stack X) : MemPropT MemState X :=
+    fun ms res =>
+      m (MemState_get_memory ms) (fmap (fun '(ms, x) => (MemState_get_memory ms, x)) res) /\
+        (* Provenance should be preserved as memory operation shouldn't touch rest of MemState *)
+        forall ms' x, res = ret (ms', x) -> MemState_get_provenance ms = MemState_get_provenance ms'.
 
   Definition byte_allocated_MemPropT (ptr : addr) (aid : AllocationId) : MemPropT MemState unit :=
-    m <- get_mem_state;;
-    b <- addr_allocated_prop ptr aid;;
+    b <- lift_memory_MemPropT (addr_allocated_prop ptr aid);;
     MemPropT_assert (b = true).
 
   Definition byte_allocated (ms : MemState) (ptr : addr) (aid : AllocationId) : Prop
@@ -1027,7 +1044,7 @@ Module Type MemoryModelSpec (LP : LLVMParams) (MP : MemoryParams LP) (MMSP : Mem
   (** Frame stack *)
   Definition frame_stack_preserved (m1 m2 : MemState) : Prop
     := forall fs,
-      mem_state_frame_stack_prop m1 fs <-> mem_state_frame_stack_prop m2 fs.
+      mem_state_frame_stack_prop (MemState_get_memory m1) fs <-> mem_state_frame_stack_prop (MemState_get_memory m2) fs.
 
   (*** Provenance operations *)
   #[global] Instance MemPropT_MonadProvenance : MonadProvenance Provenance (MemPropT MemState).
@@ -1123,7 +1140,7 @@ Module Type MemoryModelSpec (LP : LLVMParams) (MP : MemoryParams LP) (MMSP : Mem
     }.
 
   Definition ptr_in_current_frame (ms : MemState) (ptr : addr) : Prop
-    := forall fs, mem_state_frame_stack_prop ms fs ->
+    := forall fs, mem_state_frame_stack_prop (MemState_get_memory ms) fs ->
              forall f, peek_frame_stack_prop fs f ->
                   ptr_in_frame_prop f ptr.
 
@@ -1140,10 +1157,10 @@ Module Type MemoryModelSpec (LP : LLVMParams) (MP : MemoryParams LP) (MMSP : Mem
     {
       fresh_frame :
       forall fs1 fs2 f,
-        mem_state_frame_stack_prop m1 fs1 ->
+        mem_state_frame_stack_prop (MemState_get_memory m1) fs1 ->
         empty_frame f ->
         push_frame_stack_spec fs1 f fs2 ->
-        mem_state_frame_stack_prop m2 fs2;
+        mem_state_frame_stack_prop (MemState_get_memory m2) fs2;
 
       mempush_invariants :
       mempush_operation_invariants m1 m2;
@@ -1191,9 +1208,9 @@ Module Type MemoryModelSpec (LP : LLVMParams) (MP : MemoryParams LP) (MMSP : Mem
       (* Set new framestack *)
       pop_frame :
       forall fs1 fs2,
-        mem_state_frame_stack_prop m1 fs1 ->
+        mem_state_frame_stack_prop (MemState_get_memory m1) fs1 ->
         pop_frame_stack_prop fs1 fs2 ->
-        mem_state_frame_stack_prop m2 fs2;
+        mem_state_frame_stack_prop (MemState_get_memory m2) fs2;
 
       (* Invariants *)
       mempop_invariants : mempop_operation_invariants m1 m2;
@@ -1325,9 +1342,9 @@ Module Type MemoryModelSpec (LP : LLVMParams) (MP : MemoryParams LP) (MMSP : Mem
       (* Add allocated bytes onto the stack frame *)
       allocate_bytes_add_to_frame :
       forall fs1 fs2,
-        mem_state_frame_stack_prop m1 fs1 ->
+        mem_state_frame_stack_prop (MemState_get_memory m1) fs1 ->
         add_ptrs_to_frame_stack fs1 ptrs fs2 ->
-        mem_state_frame_stack_prop m2 fs2;
+        mem_state_frame_stack_prop (MemState_get_memory m2) fs2;
 
       (* Type is valid *)
       allocate_bytes_typ :
@@ -1503,7 +1520,7 @@ Module Type MemoryModelExecPrimitives (LP : LLVMParams) (MP : MemoryParams LP).
     Context {MemM : Type -> Type}.
     Context {Eff : Type -> Type}.
     Context {ExtraState : Type}.
-    Context `{MM : MemMonad MemState ExtraState Provenance MemM (itree Eff)}.
+    Context `{MM : MemMonad MemState memory_stack ExtraState Provenance MemM (itree Eff)}.
 
     (*** Data types *)
     Parameter initial_memory_state : MemState.
@@ -1512,26 +1529,33 @@ Module Type MemoryModelExecPrimitives (LP : LLVMParams) (MP : MemoryParams LP).
     (*** Primitives on memory *)
     (** Reads *)
     Parameter read_byte :
-      forall `{MemMonad MemState ExtraState Provenance MemM (itree Eff)}, addr -> MemM SByte.
+      forall `{MemMonad MemState memory_stack ExtraState Provenance MemM (itree Eff)}, addr -> MemM SByte.
 
     (** Writes *)
     Parameter write_byte :
-      forall `{MemMonad MemState ExtraState Provenance MemM (itree Eff)}, addr -> SByte -> MemM unit.
+      forall `{MemMonad MemState memory_stack ExtraState Provenance MemM (itree Eff)}, addr -> SByte -> MemM unit.
 
     (** Allocations *)
     Parameter allocate_bytes :
-      forall `{MemMonad MemState ExtraState Provenance MemM (itree Eff)}, dtyp -> list SByte -> MemM addr.
+      forall `{MemMonad MemState memory_stack ExtraState Provenance MemM (itree Eff)}, dtyp -> list SByte -> MemM addr.
 
     (** Frame stacks *)
-    Parameter mempush : forall `{MemMonad MemState ExtraState Provenance MemM (itree Eff)}, MemM unit.
-    Parameter mempop : forall `{MemMonad MemState ExtraState Provenance MemM (itree Eff)}, MemM unit.
+    Parameter mempush : forall `{MemMonad MemState memory_stack ExtraState Provenance MemM (itree Eff)}, MemM unit.
+    Parameter mempop : forall `{MemMonad MemState memory_stack ExtraState Provenance MemM (itree Eff)}, MemM unit.
 
     (*** Correctness *)
-    Parameter exec_correct : forall {MemM Eff ExtraState} `{MemMonad MemState ExtraState Provenance MemM (itree Eff)} {X} (exec : MemM X) (spec : MemPropT MemState X), Prop.
+    Parameter exec_correct : forall {MemM Eff ExtraState} `{MemMonad MemState memory_stack ExtraState Provenance MemM (itree Eff)} {X} (exec : MemM X) (spec : MemPropT MemState X), Prop.
+
+    Parameter exec_correct_memory : forall {MemM Eff ExtraState} `{MemMonad MemState memory_stack ExtraState Provenance MemM (itree Eff)} {X} (exec : MemM X) (spec : MemPropT memory_stack X), Prop.
+
+    Parameter exec_correct_lift_memory :
+      forall {X} exec (spec : MemPropT memory_stack X),
+        exec_correct_memory exec spec ->
+        exec_correct exec (lift_memory_MemPropT spec).
 
     (** Correctness of the main operations on memory *)
     Parameter read_byte_correct :
-      forall ptr, exec_correct (read_byte ptr) (read_byte_MemPropT ptr).
+      forall ptr, exec_correct_memory (read_byte ptr) (read_byte_MemPropT ptr).
 
     Parameter write_byte_correct :
       forall ptr byte, exec_correct (write_byte ptr byte) (write_byte_spec_MemPropT ptr byte).
@@ -1555,7 +1579,7 @@ Module Type MemoryModelExecPrimitives (LP : LLVMParams) (MP : MemoryParams LP).
 
         initial_memory_frame_stack :
         forall fs,
-          mem_state_frame_stack_prop initial_memory_state fs ->
+          mem_state_frame_stack_prop (MemState_get_memory initial_memory_state) fs ->
           empty_frame_stack fs;
 
         initial_memory_no_reads :
@@ -1597,22 +1621,22 @@ Module Type MemoryModelExec (LP : LLVMParams) (MP : MemoryParams LP) (MMEP : Mem
     Context {MemM : Type -> Type}.
     Context {Eff : Type -> Type}.
     Context {ExtraState : Type}.
-    Context `{MemMonad MemState ExtraState Provenance MemM (itree Eff)}.
+    Context `{MemMonad MemState memory_stack ExtraState Provenance MemM (itree Eff)}.
 
     (** Reading uvalues *)
-    Definition read_bytes `{MemMonad MemState ExtraState Provenance MemM (itree Eff)} (ptr : addr) (len : nat) : MemM (list SByte) :=
+    Definition read_bytes `{MemMonad MemState memory_stack ExtraState Provenance MemM (itree Eff)} (ptr : addr) (len : nat) : MemM (list SByte) :=
       (* TODO: this should maybe be UB and not OOM??? *)
       ptrs <- get_consecutive_ptrs ptr len;;
 
       (* Actually perform reads *)
       Util.map_monad (fun ptr => read_byte ptr) ptrs.
 
-    Definition read_uvalue `{MemMonad MemState ExtraState Provenance MemM (itree Eff)} (dt : dtyp) (ptr : addr) : MemM uvalue :=
+    Definition read_uvalue `{MemMonad MemState memory_stack ExtraState Provenance MemM (itree Eff)} (dt : dtyp) (ptr : addr) : MemM uvalue :=
       bytes <- read_bytes ptr (N.to_nat (sizeof_dtyp dt));;
       lift_err_RAISE_ERROR (deserialize_sbytes bytes dt).
 
     (** Writing uvalues *)
-    Definition write_bytes `{MemMonad MemState ExtraState Provenance MemM (itree Eff)} (ptr : addr) (bytes : list SByte) : MemM unit :=
+    Definition write_bytes `{MemMonad MemState memory_stack ExtraState Provenance MemM (itree Eff)} (ptr : addr) (bytes : list SByte) : MemM unit :=
       (* TODO: Should this be UB instead of OOM? *)
       ptrs <- get_consecutive_ptrs ptr (length bytes);;
       let ptr_bytes := zip ptrs bytes in
@@ -1620,19 +1644,19 @@ Module Type MemoryModelExec (LP : LLVMParams) (MP : MemoryParams LP) (MMEP : Mem
       (* Actually perform writes *)
       Util.map_monad_ (fun '(ptr, byte) => write_byte ptr byte) ptr_bytes.
 
-    Definition write_uvalue `{MemMonad MemState ExtraState Provenance MemM (itree Eff)} (dt : dtyp) (ptr : addr) (uv : uvalue) : MemM unit :=
+    Definition write_uvalue `{MemMonad MemState memory_stack ExtraState Provenance MemM (itree Eff)} (dt : dtyp) (ptr : addr) (uv : uvalue) : MemM unit :=
       bytes <- serialize_sbytes uv dt;;
       write_bytes ptr bytes.
 
     (** Allocating dtyps *)
     (* Need to make sure MemPropT has provenance and sids to generate the bytes. *)
-    Definition allocate_dtyp `{MemMonad MemState ExtraState Provenance MemM (itree Eff)} (dt : dtyp) : MemM addr :=
+    Definition allocate_dtyp `{MemMonad MemState memory_stack ExtraState Provenance MemM (itree Eff)} (dt : dtyp) : MemM addr :=
       sid <- fresh_sid;;
       bytes <- lift_OOM (generate_undef_bytes dt sid);;
       allocate_bytes dt bytes.
 
     (** Handle memcpy *)
-    Definition memcpy `{MemMonad MemState ExtraState Provenance MemM (itree Eff)} (src dst : addr) (len : Z) (align : N) (volatile : bool) : MemM unit :=
+    Definition memcpy `{MemMonad MemState memory_stack ExtraState Provenance MemM (itree Eff)} (src dst : addr) (len : Z) (align : N) (volatile : bool) : MemM unit :=
       if Z.ltb len 0
       then
         raise_ub "memcpy given negative length."
@@ -1651,7 +1675,7 @@ Module Type MemoryModelExec (LP : LLVMParams) (MP : MemoryParams LP) (MMEP : Mem
         else
           raise_ub "memcpy with overlapping or non-equal src and dst memory locations.".
 
-    Definition handle_memory `{MemMonad MemState ExtraState Provenance MemM (itree Eff)} : MemoryE ~> MemM
+    Definition handle_memory `{MemMonad MemState memory_stack ExtraState Provenance MemM (itree Eff)} : MemoryE ~> MemM
       := fun T m =>
            match m with
            (* Unimplemented *)
@@ -1678,7 +1702,7 @@ Module Type MemoryModelExec (LP : LLVMParams) (MP : MemoryParams LP) (MMEP : Mem
                end
            end.
 
-    Definition handle_memcpy `{MemMonad MemState ExtraState Provenance MemM (itree Eff)} (args : list dvalue) : MemM unit :=
+    Definition handle_memcpy `{MemMonad MemState memory_stack ExtraState Provenance MemM (itree Eff)} (args : list dvalue) : MemM unit :=
       match args with
       | DVALUE_Addr dst ::
                     DVALUE_Addr src ::
@@ -1701,7 +1725,7 @@ Module Type MemoryModelExec (LP : LLVMParams) (MP : MemoryParams LP) (MMEP : Mem
       | _ => raise_error "Unsupported arguments to memcpy."
       end.
 
-    Definition handle_intrinsic `{MemMonad MemState ExtraState Provenance MemM (itree Eff)} : IntrinsicE ~> MemM
+    Definition handle_intrinsic `{MemMonad MemState memory_stack ExtraState Provenance MemM (itree Eff)} : IntrinsicE ~> MemM
       := fun T e =>
            match e with
            | Intrinsic t name args =>
